firmware/Aes/AesExampleProperties.v
@@ -32,22 +32,23 @@ Import Syntax.Coercions List.ListNotations.
 Local Open Scope Z_scope.
 
 Section Proofs.
-  Context {p : AesSemantics.parameters} {p_ok : parameters.ok p}
-          {consts : aes_constants Z} {timing : timing}.
-  Context {consts_ok : aes_constants_ok consts}.
-  Existing Instance state_machine_parameters.
+  Context {word: word.word 32} {mem: map.map word Byte.byte}
+          {word_ok: word.ok word} {mem_ok: map.ok mem}
+          {ASpec: AesSpec}
+          {consts : aes_constants Z} {timing : timing}
+          {consts_ok : aes_constants_ok consts}.
   Existing Instance constant_literals.
 
-  Instance spec_of_aes_encrypt : spec_of "b2_aes_encrypt" :=
+  Global Instance spec_of_aes_encrypt : spec_of "b2_aes_encrypt" :=
     fun function_env =>
       forall (tr : trace) (m : mem) R
-        (plaintext_ptr key_ptr iv_ptr ciphertext_ptr : Semantics.word)
+        (plaintext_ptr key_ptr iv_ptr ciphertext_ptr : word)
         (* values of input arrays *)
         (plaintext0 plaintext1 plaintext2 plaintext3
                     key0 key1 key2 key3 key4 key5 key6 key7
-                    iv0 iv1 iv2 iv3 : Semantics.word)
+                    iv0 iv1 iv2 iv3 : word)
         (* initial values of output array (used only for determining length) *)
-        (ciphertext_arr : list Semantics.word),
+        (ciphertext_arr : list word),
         let plaintext_arr := [plaintext0; plaintext1; plaintext2; plaintext3] in
         let key_arr := [key0; key1; key2; key3; key4; key5; key6; key7] in
         let iv_arr := [iv0; iv1; iv2; iv3] in
@@ -60,11 +61,11 @@ Section Proofs.
         (* output array has the right length *)
         length ciphertext_arr = 4%nat ->
         (* circuit must start in the UNINITIALIZED state *)
-        execution (p:=state_machine_parameters) tr UNINITIALIZED ->
+        execution tr UNINITIALIZED ->
         (* determine expected output using aes_spec *)
         let is_decrypt := false in
         let expected_output :=
-            parameters.aes_spec
+            aes_spec
               is_decrypt
               (key0, key1, key2, key3, key4, key5, key6, key7)
               (iv0, iv1, iv2, iv3)
@@ -74,7 +75,7 @@ Section Proofs.
              (fun tr' m' rets =>
                 let '(out0, out1, out2, out3) := expected_output in
                 (* the circuit is back in the IDLE state *)
-                (exists data, execution (p:=state_machine_parameters) tr' (IDLE data))
+                (exists data, execution tr' (IDLE data))
                 (* ...and the input arrays are unchanged, while the ciphertext
                      array now holds the values from the expected output *)
                 /\ (array scalar32 (word.of_Z 4) plaintext_ptr plaintext_arr
@@ -112,8 +113,6 @@ Section Proofs.
       pose proof (enum_unique aes_key_len) as Hunique.
       simplify_unique_words_in Hunique.
       cbn [kAes256 kAes128 kAes192].
-      change Semantics.width with 32.
-      change Semantics.word with parameters.word.
       repeat destruct_one_match; subst; try congruence; [ ].
       reflexivity. }
 
@@ -155,8 +154,8 @@ Section Proofs.
     lazymatch goal with
     | Hsep : sep _ _ ?m |- sep _ _ ?m =>
       lazymatch type of Hsep with
-        context [parameters.aes_spec ?op ?keys ?iv ?plaintext] =>
-        replace (parameters.aes_spec op keys iv plaintext)
+        context [aes_spec ?op ?keys ?iv ?plaintext] =>
+        replace (aes_spec op keys iv plaintext)
         with expected_output in Hsep
       end
     end; [ ecancel_assumption | ].
